dllbc/Dllbc.lean
@@ -30,3 +30,4 @@ import Dllbc.Tests.SetHmProbe
 import Dllbc.Tests.ArrCatIota
 import Dllbc.Tests.HashMap
 import Dllbc.Tests.HashMapDiff
+import Dllbc.Tests.HashMapPin
